James C - mostly done chapter 20

isabelle/Chapter20_1_Language.thy
@@ -12,11 +12,51 @@ datatype type =
 | Void
 | Sum type type
 
+primrec type_insert :: "var => type => type"
+where "type_insert n (Tyvar v) = Tyvar (incr n v)"
+    | "type_insert n Nat = Nat"
+    | "type_insert n (Arrow e1 e2) = Arrow (type_insert n e1) (type_insert n e2)"
+    | "type_insert n (All e) = All (type_insert (next n) e)"
+    | "type_insert n Unit = Unit"
+    | "type_insert n (Prod e1 e2) = Prod (type_insert n e1) (type_insert n e2)"
+    | "type_insert n Void = Void"
+    | "type_insert n (Sum e1 e2) = Sum (type_insert n e1) (type_insert n e2)"
+
+primrec type_remove :: "var => type => type"
+where "type_remove n (Tyvar v) = Tyvar (subr n v)"
+    | "type_remove n Nat = Nat"
+    | "type_remove n (Arrow e1 e2) = Arrow (type_remove n e1) (type_remove n e2)"
+    | "type_remove n (All e) = All (type_remove (next n) e)"
+    | "type_remove n Unit = Unit"
+    | "type_remove n (Prod e1 e2) = Prod (type_remove n e1) (type_remove n e2)"
+    | "type_remove n Void = Void"
+    | "type_remove n (Sum e1 e2) = Sum (type_remove n e1) (type_remove n e2)"
+
+primrec type_subst' :: "var => type => type => type"
+where "type_subst' n e' (Tyvar v) = (if v = n then e' else Tyvar v)"
+    | "type_subst' n e' Nat = Nat"
+    | "type_subst' n e' (Arrow e1 e2) = Arrow (type_subst' n e' e1) (type_subst' n e' e2)"
+    | "type_subst' n e' (All e) = All (type_subst' (next n) (type_insert first e') e)"
+    | "type_subst' n e' Unit = Unit"
+    | "type_subst' n e' (Prod e1 e2) = Prod (type_subst' n e' e1) (type_subst' n e' e2)"
+    | "type_subst' n e' Void = Void"
+    | "type_subst' n e' (Sum e1 e2) = Sum (type_subst' n e' e1) (type_subst' n e' e2)"
+
+definition type_subst :: "var => type => type => type"
+where "type_subst n t' t = type_remove n (type_subst' n (type_insert n t') t)"
+
+lemma [simp]: "type_remove n (type_insert n e) = e"
+by (induction e arbitrary: n, simp_all)
+
+lemma [simp]: "canswap m n ==> 
+        type_insert m (type_insert n e) = type_insert (next n) (type_insert m e)"
+by (induction e arbitrary: n m, simp_all)
+
 datatype expr = 
   Var var
 | Zero
 | Suc expr
-| Rec expr expr expr
+| Iter expr expr expr
 | Lam type expr
 | Appl expr expr
 | TyLam expr
@@ -34,7 +74,7 @@ primrec insert :: "var => expr => expr"
 where "insert n (Var v) = Var (incr n v)"
     | "insert n Zero = Zero"
     | "insert n (Suc e) = Suc (insert n e)"
-    | "insert n (Rec et e0 es) = Rec (insert n et) (insert n e0) (insert (next (next n)) es)"
+    | "insert n (Iter et e0 es) = Iter (insert n et) (insert n e0) (insert (next n) es)"
     | "insert n (Lam t e) = Lam t (insert (next n) e)"
     | "insert n (Appl e1 e2) = Appl (insert n e1) (insert n e2)"
     | "insert n (TyLam e) = TyLam (insert n e)"
@@ -52,7 +92,7 @@ primrec remove :: "var => expr => expr"
 where "remove n (Var v) = Var (subr n v)"
     | "remove n Zero = Zero"
     | "remove n (Suc e) = Suc (remove n e)"
-    | "remove n (Rec et e0 es) = Rec (remove n et) (remove n e0) (remove (next (next n)) es)"
+    | "remove n (Iter et e0 es) = Iter (remove n et) (remove n e0) (remove (next n) es)"
     | "remove n (Lam t e) = Lam t (remove (next n) e)"
     | "remove n (Appl e1 e2) = Appl (remove n e1) (remove n e2)"
     | "remove n (TyLam e) = TyLam (remove n e)"
@@ -70,10 +110,10 @@ primrec subst' :: "var => expr => expr => expr"
 where "subst' n e' (Var v) = (if v = n then e' else Var v)"
     | "subst' n e' Zero = Zero"
     | "subst' n e' (Suc e) = Suc (subst' n e' e)"
-    | "subst' n e' (Rec et e0 es) = 
-                      Rec (subst' n e' et) 
-                          (subst' n e' e0) 
-                          (subst' (next (next n)) (insert first (insert first e')) es)"
+    | "subst' n e' (Iter et e0 es) = 
+                      Iter (subst' n e' et) 
+                           (subst' n e' e0) 
+                           (subst' (next n) (insert first e') es)"
     | "subst' n e' (Lam t e) = Lam t (subst' (next n) (insert first e') e)"
     | "subst' n e' (Appl e1 e2) = Appl (subst' n e' e1) (subst' n e' e2)"
     | "subst' n e' (TyLam e) = TyLam (subst' n e' e)"
@@ -98,5 +138,29 @@ by (induction e arbitrary: n, simp_all)
 
 lemma [simp]: "canswap m n ==> insert m (insert n e) = insert (next n) (insert m e)"
 by (induction e arbitrary: n m, simp_all)
+
+primrec subst_type :: "var => type => expr => expr"
+where "subst_type n t' (Var v) = Var v"
+    | "subst_type n t' Zero = Zero"
+    | "subst_type n t' (Suc e) = Suc (subst_type n t' e)"
+    | "subst_type n t' (Iter et e0 es) = 
+                      Iter (subst_type n t' et) 
+                           (subst_type n t' e0) 
+                           (subst_type n t' es)"
+    | "subst_type n t' (Lam t e) = Lam (type_subst n t' t) (subst_type n t' e)"
+    | "subst_type n t' (Appl e1 e2) = Appl (subst_type n t' e1) (subst_type n t' e2)"
+    | "subst_type n t' (TyLam e) = TyLam (subst_type (next n) (type_insert first t') e)"
+    | "subst_type n t' (TyAppl t e) = TyAppl (type_subst n t' t) (subst_type n t' e)"
+    | "subst_type n t' Triv = Triv"
+    | "subst_type n t' (Pair e1 e2) = Pair (subst_type n t' e1) (subst_type n t' e2)"
+    | "subst_type n t' (ProjL e) = ProjL (subst_type n t' e)"
+    | "subst_type n t' (ProjR e) = ProjR (subst_type n t' e)"
+    | "subst_type n t' (Abort t e) = Abort (type_subst n t' t) (subst_type n t' e)"
+    | "subst_type n t' (Case et el er) = 
+                      Case (subst_type n t' et) (subst_type n t' el) (subst_type n t' er)"
+    | "subst_type n t' (InL t1 t2 e) = 
+                      InL (type_subst n t' t1) (type_subst n t' t2) (subst_type n t' e)"
+    | "subst_type n t' (InR t1 t2 e) = 
+                      InR (type_subst n t' t1) (type_subst n t' t2) (subst_type n t' e)"
 
 end
