isabelle/Chapter20_2_Typechecking.thy
@@ -2,53 +2,156 @@ theory Chapter20_2_Typechecking
 imports Chapter20_1_Language
 begin
 
-inductive typecheck :: "type env => expr => type => bool"
-where tc_var [simp]: "lookup gam x = Some t ==> typecheck gam (Var x) t"
-    | tc_zero [simp]: "typecheck gam Zero Nat"
-    | tc_suc [simp]: "typecheck gam e Nat ==> typecheck gam (Suc e) Nat"
-    | tc_rec [simp]: "typecheck gam et Nat ==> typecheck gam e0 t ==> 
-                typecheck (extend (extend gam t) Nat) es t ==> typecheck gam (Rec et e0 es) t"
-    | tc_lam [simp]: "typecheck (extend gam t1) e t2 ==> typecheck gam (Lam t1 e) (Arrow t1 t2)"
-    | tc_appl [simp]: "typecheck gam e1 (Arrow t2 t) ==> typecheck gam e2 t2 ==> 
-                typecheck gam (Appl e1 e2) t"
-    | tc_triv [simp]: "typecheck gam Triv Unit"
-    | tc_pair [simp]: "typecheck gam e1 t1 ==> typecheck gam e2 t2 ==> 
-                typecheck gam (Pair e1 e2) (Prod t1 t2)"
-    | tc_projl [simp]: "typecheck gam e (Prod t1 t2) ==> typecheck gam (ProjL e) t1"
-    | tc_projr [simp]: "typecheck gam e (Prod t1 t2) ==> typecheck gam (ProjR e) t2"
-    | tc_abort [simp]: "typecheck gam e Void ==> typecheck gam (Abort t e) t"
-    | tc_case [simp]: "typecheck gam et (Sum t1 t2) ==> typecheck (extend gam t1) el t ==> 
-                typecheck (extend gam t2) er t ==> typecheck gam (Case et el er) t"
-    | tc_inl [simp]: "typecheck gam e t1 ==> typecheck gam (InL t1 t2 e) (Sum t1 t2)"
-    | tc_inr [simp]: "typecheck gam e t2 ==> typecheck gam (InR t1 t2 e) (Sum t1 t2)"
+primrec is_type :: "var => type => bool"
+where "is_type del (Tyvar v) = canswap v del"
+    | "is_type del Nat = True"
+    | "is_type del (Arrow e1 e2) = (is_type del e1 & is_type del e2)"
+    | "is_type del (All e) = is_type (next del) e"
+    | "is_type del Unit = True"
+    | "is_type del (Prod e1 e2) = (is_type del e1 & is_type del e2)"
+    | "is_type del Void = True"
+    | "is_type del (Sum e1 e2) = (is_type del e1 & is_type del e2)"
 
-inductive_cases [elim!]: "typecheck gam (Var x) t"
-inductive_cases [elim!]: "typecheck gam Zero t"
-inductive_cases [elim!]: "typecheck gam (Suc e) t"
-inductive_cases [elim!]: "typecheck gam (Rec et e0 es) t"
-inductive_cases [elim!]: "typecheck gam (Lam t1 e) t"
-inductive_cases [elim!]: "typecheck gam (Appl e1 e2) t"
-inductive_cases [elim!]: "typecheck gam (TyLam e) t"
-inductive_cases [elim!]: "typecheck gam (TyAppl e1 e2) t"
-inductive_cases [elim!]: "typecheck gam Triv t"
-inductive_cases [elim!]: "typecheck gam (Pair e1 e2) t"
-inductive_cases [elim!]: "typecheck gam (ProjL e) t"
-inductive_cases [elim!]: "typecheck gam (ProjR e) t"
-inductive_cases [elim!]: "typecheck gam (Abort t1 e) t"
-inductive_cases [elim!]: "typecheck gam (Case et el er) t"
-inductive_cases [elim!]: "typecheck gam (InL t1 t2 e) t"
-inductive_cases [elim!]: "typecheck gam (InR t1 t2 e) t"
+inductive typecheck :: "var => type env => expr => type => bool"
+where tc_var [simp]: "lookup gam x = Some t ==> typecheck del gam (Var x) t"
+    | tc_zero [simp]: "typecheck del gam Zero Nat"
+    | tc_suc [simp]: "typecheck del gam e Nat ==> typecheck del gam (Suc e) Nat"
+    | tc_rec [simp]: "typecheck del gam et Nat ==> typecheck del gam e0 t ==> 
+                typecheck del (extend gam t) es t ==> typecheck del gam (Iter et e0 es) t"
+    | tc_lam [simp]: "is_type del t1 ==> typecheck del (extend gam t1) e t2 ==> 
+                typecheck del gam (Lam t1 e) (Arrow t1 t2)"
+    | tc_appl [simp]: "typecheck del gam e1 (Arrow t2 t) ==> typecheck del gam e2 t2 ==> 
+                typecheck del gam (Appl e1 e2) t"
+    | tc_tylam [simp]: "typecheck (next del) gam e t ==> typecheck del gam (TyLam e) (All t)"
+    | tc_tyappl [simp]: "is_type del t' ==> typecheck del gam e (All t) ==> 
+                typecheck del gam (TyAppl t' e) (type_subst first t' t)"
+    | tc_triv [simp]: "typecheck del gam Triv Unit"
+    | tc_pair [simp]: "typecheck del gam e1 t1 ==> typecheck del gam e2 t2 ==> 
+                typecheck del gam (Pair e1 e2) (Prod t1 t2)"
+    | tc_projl [simp]: "typecheck del gam e (Prod t1 t2) ==> typecheck del gam (ProjL e) t1"
+    | tc_projr [simp]: "typecheck del gam e (Prod t1 t2) ==> typecheck del gam (ProjR e) t2"
+    | tc_abort [simp]: "is_type del t ==> typecheck del gam e Void ==> 
+                typecheck del gam (Abort t e) t"
+    | tc_case [simp]: "typecheck del gam et (Sum t1 t2) ==> typecheck del (extend gam t1) el t ==> 
+                typecheck del (extend gam t2) er t ==> typecheck del gam (Case et el er) t"
+    | tc_inl [simp]: "is_type del t1 ==> is_type del t2 ==> typecheck del gam e t1 ==> 
+                typecheck del gam (InL t1 t2 e) (Sum t1 t2)"
+    | tc_inr [simp]: "is_type del t1 ==> is_type del t2 ==> typecheck del gam e t2 ==> 
+                typecheck del gam (InR t1 t2 e) (Sum t1 t2)"
 
-lemma [simp]: "typecheck gam e t ==> n in gam ==> 
-         typecheck (extend_at n gam t') (insert n e) t"
-by (induction gam e t arbitrary: n rule: typecheck.induct, fastforce+)
+inductive_cases [elim!]: "typecheck del gam (Var x) t"
+inductive_cases [elim!]: "typecheck del gam Zero t"
+inductive_cases [elim!]: "typecheck del gam (Suc e) t"
+inductive_cases [elim!]: "typecheck del gam (Iter et e0 es) t"
+inductive_cases [elim!]: "typecheck del gam (Lam t1 e) t"
+inductive_cases [elim!]: "typecheck del gam (Appl e1 e2) t"
+inductive_cases [elim!]: "typecheck del gam (TyLam e) t"
+inductive_cases [elim!]: "typecheck del gam (TyAppl e1 e2) t"
+inductive_cases [elim!]: "typecheck del gam Triv t"
+inductive_cases [elim!]: "typecheck del gam (Pair e1 e2) t"
+inductive_cases [elim!]: "typecheck del gam (ProjL e) t"
+inductive_cases [elim!]: "typecheck del gam (ProjR e) t"
+inductive_cases [elim!]: "typecheck del gam (Abort t1 e) t"
+inductive_cases [elim!]: "typecheck del gam (Case et el er) t"
+inductive_cases [elim!]: "typecheck del gam (InL t1 t2 e) t"
+inductive_cases [elim!]: "typecheck del gam (InR t1 t2 e) t"
 
-lemma [simp]: "typecheck (extend_at n gam t') e t ==> n in gam ==> typecheck gam e' t' ==> 
-        typecheck gam (remove n (subst' n (insert n e') e)) t"
-by (induction "extend_at n gam t'" e t arbitrary: n gam t' e' rule: typecheck.induct, fastforce+)
+lemma [simp]: "typecheck del gam e t ==> n in gam ==> 
+         typecheck del (extend_at n gam t') (insert n e) t"
+by (induction del gam e t arbitrary: n rule: typecheck.induct, fastforce+)
 
-lemma [simp]: "typecheck (extend gam t') e t ==> typecheck gam e' t' ==> 
-                          typecheck gam (subst e' e) t"
+lemma [simp]: "is_type del t ==> is_type (next del) t"
+by (induction t arbitrary: del, simp_all)
+
+lemma [simp]: "typecheck del gam e t ==> typecheck (next del) gam e t"
+by (induction del gam e t rule: typecheck.induct, simp_all)
+
+lemma [simp]: "typecheck del (extend_at n gam t') e t ==> n in gam ==> typecheck del gam e' t' ==> 
+        typecheck del gam (remove n (subst' n (insert n e') e)) t"
+by (induction del "extend_at n gam t'" e t arbitrary: n gam t' e' rule: typecheck.induct, fastforce+)
+
+lemma [simp]: "typecheck del (extend gam t') e t ==> typecheck del gam e' t' ==> 
+                          typecheck del gam (subst e' e) t"
 by (simp add: subst_def)
+
+lemma [simp]: "is_type del t ==> is_type (next del) (type_insert n t)"
+by (induction t arbitrary: n del, simp_all)
+
+lemma [simp]: "is_type (next del) t ==> is_type del t' ==> 
+                is_type del (type_remove n (type_subst' n (type_insert n t') t))"
+proof (induction t arbitrary: n del t')
+case (Tyvar v) 
+  thus ?case by simp sorry
+next case Nat 
+  thus ?case by simp
+next case (Arrow e1 e2)
+  thus ?case by simp
+next case (All e) 
+  thus ?case by simp
+next case Unit 
+  thus ?case by simp
+next case (Prod e1 e2) 
+  thus ?case by simp
+next case Void 
+  thus ?case by simp
+next case (Sum e1 e2) 
+  thus ?case by simp
+qed 
+
+lemma [simp]: "is_type (next del) t ==> is_type del t' ==> is_type del (type_subst first t' t)"
+by (simp add: type_subst_def)
+
+lemma [simp]: "typecheck (next del) gam e t ==> 
+        typecheck del (env_map (%t. type_remove n (type_subst' n (type_insert n t') t)) gam) 
+                  (subst_type n t' e) 
+                  (type_remove n (type_subst' n (type_insert n t') t))"
+proof (induction "next del" gam e t arbitrary: del t' n rule: typecheck.induct)
+case tc_var
+  thus ?case by simp
+next case tc_zero
+  thus ?case by simp
+next case tc_suc
+  thus ?case by simp
+next case (tc_rec gam et e0 t es)
+  thus ?case by simp sorry
+next case (tc_lam gam t1 e t2)
+  thus ?case by simp sorry
+next case (tc_appl gam e1 t2 t e2)
+  thus ?case by simp sorry
+next case (tc_tylam gam e t)
+  thus ?case by simp sorry
+next case (tc_tyappl gam e t t2)
+  thus ?case by simp sorry
+next case tc_triv
+  thus ?case by simp
+next case tc_pair
+  thus ?case by simp
+next case tc_projl
+  thus ?case 
+  by (metis subst_type.simps(11) type_remove.simps(6) type_subst'.simps(6) typecheck.tc_projl)
+next case tc_projr
+  thus ?case 
+  by (metis subst_type.simps(12) type_remove.simps(6) type_subst'.simps(6) typecheck.tc_projr)
+next case (tc_abort t gam e)
+  from tc_abort have "is_type (next del) t" by simp
+  from tc_abort have "typecheck (next del) gam e Void" by simp
+
+  have X: "is_type del (type_subst n t' t)" by simp sorry
+  with tc_abort show ?case by (simp add: type_subst_def)
+next case tc_case
+  thus ?case by simp sorry
+next case tc_inl
+  thus ?case by simp sorry
+next case tc_inr
+  thus ?case by simp sorry
+qed
+
+lemma [simp]: "typecheck (next del) gam e t ==> 
+        typecheck del (env_map (%v. type_subst n t' v) gam) (subst_type n t' e) (type_subst n t' t)"
+by (simp add: type_subst_def)
+
+lemma [simp]: "typecheck (next del) gam e t ==> 
+        typecheck del (env_map (type_subst n t') gam) (subst_type n t' e) (type_subst n t' t)"
+by auto
 
 end
