isabelle/Chapter20_3_Evaluation.thy
@@ -6,7 +6,7 @@ primrec is_val :: "expr => bool"
 where "is_val (Var v) = False"
     | "is_val Zero = True"
     | "is_val (Suc e) = is_val e"
-    | "is_val (Rec et e0 es) = False"
+    | "is_val (Iter et e0 es) = False"
     | "is_val (Lam t e) = True"
     | "is_val (Appl e1 e2) = False"
     | "is_val (TyLam e) = True"
@@ -22,13 +22,14 @@ where "is_val (Var v) = False"
 
 inductive eval :: "expr => expr => bool"
 where eval_suc [simp]: "eval e e' ==> eval (Suc e) (Suc e')"
-    | eval_rec_1 [simp]: "eval et et' ==> eval (Rec et e0 es) (Rec et' e0 es)"
-    | eval_rec_2 [simp]: "eval (Rec Zero e0 es) e0"
-    | eval_rec_3 [simp]: "is_val et ==> 
-            eval (Rec (Suc et) e0 es) (subst (Rec et e0 es) (subst et es))"
+    | eval_rec_1 [simp]: "eval et et' ==> eval (Iter et e0 es) (Iter et' e0 es)"
+    | eval_rec_2 [simp]: "eval (Iter Zero e0 es) e0"
+    | eval_rec_3 [simp]: "is_val et ==> eval (Iter (Suc et) e0 es) (subst (Iter et e0 es) es)"
     | eval_appl_1 [simp]: "eval e1 e1' ==> eval (Appl e1 e2) (Appl e1' e2)"
     | eval_appl_2 [simp]: "is_val e1 ==> eval e2 e2' ==> eval (Appl e1 e2) (Appl e1 e2')"
     | eval_appl_3 [simp]: "is_val e2 ==> eval (Appl (Lam t2 e1) e2) (subst e2 e1)"
+    | eval_tyappl_1 [simp]: "eval e e' ==> eval (TyAppl t e) (TyAppl t e')"
+    | eval_tyappl_2 [simp]: "eval (TyAppl t (TyLam e)) (subst_type first t e)"
     | eval_pair_1 [simp]: "eval e1 e1' ==> eval (Pair e1 e2) (Pair e1' e2)"
     | eval_pair_2 [simp]: "is_val e1 ==> eval e2 e2' ==> eval (Pair e1 e2) (Pair e1 e2')"
     | eval_projl_1 [simp]: "eval e e' ==> eval (ProjL e) (ProjL e')"
@@ -42,49 +43,61 @@ where eval_suc [simp]: "eval e e' ==> eval (Suc e) (Suc e')"
     | eval_inl [simp]: "eval e e' ==> eval (InL t1 t2 e) (InL t1 t2 e')"
     | eval_inr [simp]: "eval e e' ==> eval (InR t1 t2 e) (InR t1 t2 e')"
 
-lemma canonical_nat: "is_val e ==> typecheck gam e Nat ==> 
-          e = Zero | (EX e'. e = Suc e' & typecheck gam e' Nat)"
+lemma canonical_nat: "is_val e ==> typecheck del gam e Nat ==> 
+          e = Zero | (EX e'. e = Suc e' & typecheck del gam e' Nat)"
 by (induction e, auto)
 
-lemma canonical_nat_no_vars: "is_val e ==> typecheck gam e Nat ==> typecheck gam' e Nat"
+lemma canonical_nat_no_vars: "is_val e ==> typecheck del gam e Nat ==> typecheck del gam' e Nat"
 by (induction e, auto) 
 
-lemma canonical_arrow: "is_val e ==> typecheck gam e (Arrow t1 t2) ==> 
-              EX e'. e = Lam t1 e' & typecheck (extend gam t1) e' t2"
+lemma canonical_arrow: "is_val e ==> typecheck del gam e (Arrow t1 t2) ==> 
+              EX e'. e = Lam t1 e' & typecheck del (extend gam t1) e' t2"
 by (induction e, auto)
 
-lemma canonical_unit: "is_val e ==> typecheck gam e Unit ==> e = Triv"
+lemma canonical_all: "is_val e ==> typecheck del gam e (All t) ==> 
+              EX e'. e = TyLam e' & typecheck (next del) gam e' t"
 by (induction e, auto)
 
-lemma canonical_prod: "is_val e ==> typecheck gam e (Prod t1 t2) ==> 
-              EX e1 e2. e = Pair e1 e2 & typecheck gam e1 t1 & typecheck gam e2 t2"
+lemma canonical_unit: "is_val e ==> typecheck del gam e Unit ==> e = Triv"
 by (induction e, auto)
 
-lemma canonical_void: "is_val e ==> typecheck gam e Void ==> False"
+lemma canonical_prod: "is_val e ==> typecheck del gam e (Prod t1 t2) ==> 
+              EX e1 e2. e = Pair e1 e2 & typecheck del gam e1 t1 & typecheck del gam e2 t2"
 by (induction e, auto)
 
-lemma canonical_sum: "is_val e ==> typecheck gam e (Sum t1 t2) ==> 
-          (EX e'. e = InL t1 t2 e' & typecheck gam e' t1) | 
-          (EX e'. e = InR t1 t2 e' & typecheck gam e' t2)"
+lemma canonical_void: "is_val e ==> typecheck del gam e Void ==> False"
 by (induction e, auto)
 
-theorem preservation: "eval e e' ==> typecheck gam e t ==> typecheck gam e' t"
+lemma canonical_sum: "is_val e ==> typecheck del gam e (Sum t1 t2) ==> 
+          (EX e'. e = InL t1 t2 e' & typecheck del gam e' t1) | 
+          (EX e'. e = InR t1 t2 e' & typecheck del gam e' t2)"
+by (induction e, auto)
+
+theorem preservation: "eval e e' ==> gam = empty_env ==> 
+          typecheck del gam e t ==> typecheck del gam e' t"
 proof (induction e e' arbitrary: t rule: eval.induct)
 case eval_suc 
   thus ?case by fastforce
-next case eval_rec_1 
+next case eval_rec_1
   thus ?case by fastforce
 next case eval_rec_2 
   thus ?case by fastforce
-next case (eval_rec_3 et e0 es)
-  from eval_rec_3 canonical_nat_no_vars have "typecheck (extend gam t) (subst et es) t" by auto
-  with eval_rec_3 show ?case by fastforce
+next case eval_rec_3
+  thus ?case by fastforce
 next case eval_appl_1 
   thus ?case by fastforce
 next case eval_appl_2 
   thus ?case by fastforce
 next case eval_appl_3 
   thus ?case by fastforce
+next case eval_tyappl_1 
+  thus ?case by fastforce
+next case (eval_tyappl_2 t' e)
+  then obtain tt where TT: "typecheck (next del) gam e tt & t = type_subst first t' tt" by force
+  hence "typecheck del (env_map (type_subst first t') gam) 
+                       (subst_type first t' e) 
+                       (type_subst first t' tt)" by simp
+  with eval_tyappl_2 TT show ?case by simp
 next case eval_pair_1 
   thus ?case by fastforce
 next case eval_pair_2 
@@ -111,7 +124,8 @@ next case eval_inr
   thus ?case by fastforce
 qed
 
-theorem progress: "typecheck gam e t ==> gam = empty_env ==> is_val e | (EX e'. eval e e')"
+theorem progress: "typecheck del gam e t ==> gam = empty_env ==>
+          is_val e | (EX e'. eval e e')"
 proof (induction gam e t rule: typecheck.induct)
 case tc_var
   thus ?case by simp
@@ -125,6 +139,10 @@ next case tc_lam
   thus ?case by simp
 next case tc_appl
   thus ?case by (metis eval_appl_1 eval_appl_2 eval_appl_3 canonical_arrow)
+next case tc_tylam
+  thus ?case by simp
+next case tc_tyappl
+  thus ?case by (metis eval_tyappl_1 eval_tyappl_2 canonical_all)
 next case tc_triv
   thus ?case by simp
 next case tc_pair
@@ -137,7 +155,7 @@ next case tc_abort
   thus ?case by (metis eval_abort canonical_void)
 next case tc_case
   thus ?case 
-  by (metis eval_case_1 eval_case_2 eval_case_3 is_val.simps(15) is_val.simps(16) canonical_sum)
+  by (metis canonical_sum eval_case_1 eval_case_2 eval_case_3 is_val.simps(15) is_val.simps(16))
 next case tc_inl
   thus ?case by (metis eval_inl is_val.simps(15))
 next case tc_inr
